theories/LogicalRelation/Definition/W.v
@@ -1,7 +1,7 @@
 (** * LogRel.LogicalRelation.Definition.Sig : Definition of the logical relation for dependent sums *)
 From Coq Require Import CRelationClasses.
 From LogRel Require Import Utils Syntax.All GenericTyping.
-From LogRel.LogicalRelation.Definition Require Import Prelude Poly Ne.
+From LogRel.LogicalRelation.Definition Require Import Prelude Poly Ne Pi.
 
 Set Primitive Projections.
 Set Universe Polymorphism.
@@ -27,6 +27,13 @@ Section WRedTmEq.
     `{Typing ta} `{ConvTerm ta} `{ConvNeuConv ta} `{RedTerm ta}
     {Γ : context} {A B : term} {WA : WRedTyPack Γ A B}.
 
+
+  Notation ContRedTm ρ a Ra wred k :=
+    (ArrRedTm _ (WRedTyPack.codL WA)[a .: ρ >> tRel] (WRedTyPack.outTy WA)⟨ρ⟩
+      (fun Ξ ρ' wfΞ => LRPack.eqTm (WA.(PolyRedPack.posRed) (ρ' ∘w ρ) wfΞ (Ra ρ' wfΞ)))
+      wred k).
+
+
   Inductive WRedTmEq {Δ} {ρ : Δ ≤ Γ} : term -> term -> Type :=
   | Build_WRedTmEq {t u}
       (nfL : term)
@@ -34,27 +41,101 @@ Section WRedTmEq.
       (redL : [ Δ |- t :⤳*: nfL : (WRedTyPack.outTy WA)⟨ρ⟩ ])
       (redR : [ Δ |- u :⤳*: nfR : (WRedTyPack.outTy WA)⟨ρ⟩ ])
       (* really useful ? *)
-      (eq : [ Γ |- nfL ≅ nfR : (WRedTyPack.outTy WA)⟨ρ⟩ ])
+      (eq : [ Δ |- nfL ≅ nfR : (WRedTyPack.outTy WA)⟨ρ⟩ ])
       (prop : @WPropEq Δ ρ nfL nfR) : WRedTmEq t u
 
   with WPropEq {Δ} {ρ : Δ ≤ Γ} : term -> term -> Type :=
   | supReq {A A' B B' a a' k k'}
     (* (wtA : [Γ |- A])
-    (wtA' : [Γ |- A']) *)
-    (convtyA : [Γ |- WRedTyPack.domL WA ≅ A])
-    (convtyA' : [Γ |- WRedTyPack.domL WA ≅ A'])
-    (convtyB : [Γ ,, WRedTyPack.domL WA |- WRedTyPack.codL WA ≅ B])
-    (convtyB' : [Γ ,, WRedTyPack.domL WA |- WRedTyPack.codL WA ≅ B'])
+    (wtA' : [Γ |- A'])
+    (wtB : [Γ,, A |- B])
+    (wtB : [Γ,, A' |- B']) *)
+    (convtyA : [Δ |- (WRedTyPack.domL WA)⟨ρ⟩ ≅ A])
+    (convtyA' : [Δ |- (WRedTyPack.domL WA)⟨ρ⟩ ≅ A'])
+    (* (convtyB : [Γ ,, WRedTyPack.domL WA |- WRedTyPack.codL WA ≅ B])
+    (convtyB' : [Γ ,, WRedTyPack.domL WA |- WRedTyPack.codL WA ≅ B']) *)
+    (* (convtyBa : [Γ |- (WRedTyPack.codL WA)[a..] ≅ B[a..]])
+    (convtyBa' : [Γ |- (WRedTyPack.codL WA)[a..] ≅ B'[a'..]]) *)
     (Ra : forall {Ξ} (ρ' : Ξ ≤ Δ) (wfΞ : [ |- Ξ ]),
       [WA.(PolyRedPack.shpRed) (ρ' ∘w ρ) wfΞ | _ ||- a⟨ρ'⟩ ≅ a'⟨ρ'⟩ : _ ≅ _])
-    (Rk : forall {Ξ b b'} (ρ' : Ξ ≤ Δ) (wfΞ : [ |- Ξ ]),
+    (* (PW := mkPolyRedPackWk1 (instPos WA ρ (@Ra)) (fun Ξ ρ' wfΞ => Build_LRPack Ξ (WRedTyPack.outTy WA)⟨ρ⟩⟨ρ'⟩ (WRedTyPack.outTy WA)⟨ρ⟩⟨ρ'⟩  (@WPropEq _ (ρ' ∘w ρ))))
+    (Rk : PiRedTm PW k) *)
+    (* (Rk : ArrRedTm Δ (WRedTyPack.domL WA) (WRedTyPack.codL WA)
+     (fun Ξ ρ' wfΞ => LRPack.eqTm (WA.(PolyRedPack.posRed) (ρ' ∘w ρ) wfΞ (Ra ρ' wfΞ)))
+     (fun Ξ ρ' wfΞ => @WPropEq _ (ρ' ∘w ρ)) k) *)
+    (Rk : ContRedTm ρ a Ra (fun Ξ ρ' wfΞ => @WRedTmEq _ (ρ' ∘w ρ)) k)
+    (Rk' : ContRedTm ρ a Ra (fun Ξ ρ' wfΞ => @WRedTmEq _ (ρ' ∘w ρ)) k')
+    (Rkk' : forall {Ξ b b'} (ρ' : Ξ ≤ Δ) (wfΞ : [ |- Ξ ]),
       [WA.(PolyRedPack.posRed) (ρ' ∘w ρ) wfΞ (Ra ρ' wfΞ) | _ ||- b ≅ b' : _ ≅ _] ->
       @WRedTmEq Ξ (ρ' ∘w ρ) (tApp k⟨ρ'⟩ b) (tApp k'⟨ρ'⟩ b')) :
     WPropEq (tSup A B a k) (tSup A' B' a' k')
   | neReq {ne ne'} :
-    [Γ ||-NeNf ne ≅ ne' : (WRedTyPack.outTy WA)⟨ρ⟩] -> WPropEq ne ne'.
+    [Δ ||-NeNf ne ≅ ne' : (WRedTyPack.outTy WA)⟨ρ⟩] -> WPropEq ne ne'.
 
-Scheme WRedTmEq_mut_rect := Induction for WRedTmEq Sort Type with
+
+  Definition ContRedTmε
+    (P : forall [Δ] (ρ : Δ ≤ Γ) [t u], @WRedTmEq _ ρ t u -> Type)
+    [Δ] (ρ : Δ ≤ Γ) [a a']
+    (Ra : forall {Ξ} (ρ' : Ξ ≤ Δ) (wfΞ : [ |- Ξ ]), [WA.(PolyRedPack.shpRed) (ρ' ∘w ρ) wfΞ | _ ||- a⟨ρ'⟩ ≅ a'⟨ρ'⟩ : _ ≅ _])
+    [k] (Rk : ContRedTm ρ a Ra (fun Ξ ρ' wfΞ => @WRedTmEq _ (ρ' ∘w ρ)) k) : Type.
+  Proof.
+    destruct Rk as [?? [???? Rt|]]; [| exact unit].
+    refine (forall [Ξ b b'] (ρ' : Ξ ≤ Δ) (wfΞ : [|- Ξ])
+      (Rb : [PolyRedPack.posRed WA (ρ' ∘w ρ) wfΞ (Ra Ξ ρ' wfΞ) | _ ||- b ≅ b' : _ ≅ _]), _).
+    eapply P, Rt, Rb.
+  Defined.
+
+  Section Eliminator.
+    Context
+      (P : forall [Δ] (ρ : Δ ≤ Γ) [t u], @WRedTmEq _ ρ t u -> Type)
+      (Q : forall [Δ] (ρ : Δ ≤ Γ) [t u], @WPropEq _ ρ t u -> Type)
+      (hred : forall [Δ] (ρ : Δ ≤ Γ) [t u] nfL nfR redL redR eq (prop : @WPropEq Δ ρ nfL nfR),
+        Q ρ prop -> @P _ ρ t u (Build_WRedTmEq nfL nfR redL redR eq prop))
+      (hne : forall [Δ] (ρ : Δ ≤ Γ) ne ne' (Rne : [Δ ||-NeNf ne ≅ ne' : (WRedTyPack.outTy WA)⟨ρ⟩]),
+        Q ρ (neReq Rne))
+      (hsup : forall [Δ] (ρ : Δ ≤ Γ) {A A' B B' a a' k k'}
+        (convtyA : [Δ |- (WRedTyPack.domL WA)⟨ρ⟩ ≅ A])
+        (convtyA' : [Δ |- (WRedTyPack.domL WA)⟨ρ⟩ ≅ A'])
+        (Ra : forall {Ξ} (ρ' : Ξ ≤ Δ) (wfΞ : [ |- Ξ ]), [WA.(PolyRedPack.shpRed) (ρ' ∘w ρ) wfΞ | _ ||- a⟨ρ'⟩ ≅ a'⟨ρ'⟩ : _ ≅ _])
+        (Rk : ContRedTm ρ a Ra (fun Ξ ρ' wfΞ => @WRedTmEq _ (ρ' ∘w ρ)) k)
+        (Rk' : ContRedTm ρ a Ra (fun Ξ ρ' wfΞ => @WRedTmEq _ (ρ' ∘w ρ)) k')
+        (Rkk' : forall {Ξ b b'} (ρ' : Ξ ≤ Δ) (wfΞ : [ |- Ξ ]),
+          [WA.(PolyRedPack.posRed) (ρ' ∘w ρ) wfΞ (Ra ρ' wfΞ) | _ ||- b ≅ b' : _ ≅ _] ->
+          @WRedTmEq Ξ (ρ' ∘w ρ) (tApp k⟨ρ'⟩ b) (tApp k'⟨ρ'⟩ b')),
+        ContRedTmε P ρ (@Ra) Rk ->
+        ContRedTmε P ρ (@Ra) Rk' ->
+        (forall Ξ b b' (ρ' : Ξ ≤ Δ) (wfΞ : [|- Ξ]) (Rb : [WA.(PolyRedPack.posRed) (ρ' ∘w ρ) wfΞ (Ra ρ' wfΞ) | _ ||- b ≅ b' : _ ≅ _]),
+          P (ρ' ∘w ρ) (Rkk' ρ' wfΞ Rb)) ->
+        Q ρ (supReq (B:=B) (B':=B') convtyA convtyA' (@Ra) Rk Rk' (@Rkk'))).
+
+    Arguments P [_] _ [_ _].
+    Arguments Q [_] _ [_ _].
+
+    Fixpoint WRedTmEq_mut_rect [Δ] (ρ : Δ ≤ Γ) [t t'] (Rt : @WRedTmEq _ ρ t t') : P ρ Rt
+    with WPropEq_mut_rect [Δ] (ρ : Δ ≤ Γ) [t t'] (Rt : @WPropEq _ ρ t t') : Q ρ Rt.
+    Proof.
+      all: destruct Rt.
+      - apply hred, WPropEq_mut_rect.
+      - apply hsup.
+        + unfold ContRedTmε; destruct Rk as [?? isfun]; destruct isfun; [|easy].
+          intros; apply WRedTmEq_mut_rect.
+        + unfold ContRedTmε; destruct Rk' as [?? isfun]; destruct isfun; [|easy].
+          intros; apply WRedTmEq_mut_rect.
+        + intros; apply WRedTmEq_mut_rect.
+      - apply hne.
+    Defined.
+
+  Let WRedEqInductionType0 :=
+    (forall Δ (ρ : Δ ≤ Γ) [t t'] (Rt : @WRedTmEq _ ρ t t'), P ρ Rt) ×
+    (forall Δ (ρ : Δ ≤ Γ) [t t'] (Rt : @WPropEq _ ρ t t'), Q ρ Rt).
+
+  Definition WRedEqInductionType := WRedEqInductionType0.
+  Definition WRedEqInduction : WRedEqInductionType0 := (@WRedTmEq_mut_rect, @WPropEq_mut_rect).
+
+  End Eliminator.
+
+
+(* Scheme WRedTmEq_mut_rect := Induction for WRedTmEq Sort Type with
     WPropEq_mut_rect := Induction for WPropEq Sort Type.
 
 Combined Scheme _WRedInduction from
@@ -81,7 +162,7 @@ Let WRedEqInductionType :=
 Lemma WRedEqInduction : WRedEqInductionType.
 Proof.
   intros PRedEq PPropEq **; split; now apply (_WRedEqInduction PRedEq PPropEq).
-Defined.
+Defined. *)
 
 End WRedTmEq.
 Arguments WRedTmEq {_ _ _ _ _ _ _ _ _ _ _ _} _ {_}.
