theories/LogicalRelation/InstKripke.v
@@ -82,40 +82,6 @@ Proof.
   intros; unshelve eapply irrLR, eq; tea; now eapply irrLRSym.
 Qed.
 
-Lemma instKripkeSubst {Γ A A' B B' l}
-  {hA : forall Δ (ρ : Δ ≤ Γ) (wfΔ : [|-Δ]), [Δ ||-<l> A⟨ρ⟩ ≅ A'⟨ρ⟩]}
-  (hB : forall Δ a b (ρ : Δ ≤ Γ) (wfΔ : [|-Δ])
-    (hab : [hA Δ ρ wfΔ | Δ ||- a ≅ b : _]),
-    [Δ ||-<l> B[a .: ρ >> tRel] ≅ B'[b .: ρ >> tRel]])
-  (RA : [Γ ||-<l> A ≅ A'])
-  [t t']
-  (ht : [_ ||-<l> t ≅ t' : _ | RA])
-  : [ Γ ||-<l> B[t..] ≅ B'[t'..]].
-Proof.
-  erewrite 2!eq_subst_scons; unshelve eapply hB.
-  2:rewrite 2! wk_id_ren_on; eapply irrLREq; tea; now rewrite wk_id_ren_on.
-  escape; gtyping.
-Qed.
-
-Lemma instKripkeSubstTm {Γ A A' B B' u u' l}
-  {hA : forall Δ (ρ : Δ ≤ Γ) (wfΔ : [|-Δ]), [Δ ||-<l> A⟨ρ⟩ ≅ A'⟨ρ⟩]}
-  {hB : forall Δ a b (ρ : Δ ≤ Γ) (wfΔ : [|-Δ])
-    (hab : [hA Δ ρ wfΔ | Δ ||- a ≅ b : _]),
-    [Δ ||-<l> B[a .: ρ >> tRel] ≅ B'[b .: ρ >> tRel]]}
-  (eq : forall Δ a b (ρ : Δ ≤ Γ) (wfΔ : [|-Δ])
-    (hab : [hA Δ ρ wfΔ | Δ ||- a ≅ b : _]),
-    [hB Δ a b ρ wfΔ hab | Δ ||- u[a .: ρ >> tRel] ≅ u'[b .: ρ >> tRel] : _])
-  (RA : [Γ ||-<l> A ≅ A'])
-  [t t' ]
-  (ht : [_ ||-<l> t ≅ t' : _ | RA])
-  : [ _ ||-<l> u[t..] ≅ u'[t'..] : _ | instKripkeSubst hB RA ht].
-Proof.
-  erewrite 2!eq_subst_scons; eapply irrLREq.
-  2: unshelve eapply eq.
-  1: now rewrite <-eq_subst_scons.
-  2: rewrite 2!wk_id_ren_on; eapply irrLREq; tea; now rewrite wk_id_ren_on.
-  escape; gtyping.
-Qed.
 
 End InstKripke.
 
